theories/Translation.v
@@ -1,3 +1,4 @@
 Require Coq.Strings.String.
-Require Template.Ast Template.tsl_fun Template.translation_utils.
+Require Template.Ast Template.translation_utils.
+Require Template.tsl_fun Template.tsl_param.
 Declare ML Module "translation_plugin".
